simpler api

docs/java/BuildTest.java
@@ -1,27 +1,35 @@
-import java.security.SecureRandom;
 import java.math.BigInteger;
 import java.util.Arrays;
-
-import DafnyVMC.Random;
-import Uniform.Interface.TraitMinus;
-import Uniform.Interface.Trait;
 
 public class BuildTest {
     public static void main(String[] args) {
         BigInteger[] arr1 = {BigInteger.valueOf(0), BigInteger.valueOf(1), BigInteger.valueOf(2)};
-        BigInteger[] arr1b = {BigInteger.valueOf(0), BigInteger.valueOf(1), BigInteger.valueOf(2)};
+        BigInteger[] arr1_custom = {BigInteger.valueOf(0), BigInteger.valueOf(1), BigInteger.valueOf(2)};
+        BigInteger[] arr1_faulty = {BigInteger.valueOf(0), BigInteger.valueOf(1), BigInteger.valueOf(2)};
         int[] arr2 = {0, 1, 2};
+        int[] arr2_custom = {0, 1, 2};
+        int[] arr2_faulty = {0, 1, 2};
         String[] arr3 = {"aa", "bb", "cc"};
+        String[] arr3_custom = {"aa", "bb", "cc"};
+        String[] arr3_faulty = {"aa", "bb", "cc"};
         char[] arr4 = {'a', 'b', 'c'};
+        char[] arr4_custom = {'a', 'b', 'c'};
+        char[] arr4_faulty = {'a', 'b', 'c'};
         boolean[] arr5 = {true, false, false, true};
+        boolean[] arr5_custom = {true, false, false, true};
+        boolean[] arr5_faulty = {true, false, false, true};
         long[] arr6 = {111111L, 333333L, 999999L};
+        long[] arr6_custom = {111111L, 333333L, 999999L};
+        long[] arr6_faulty = {111111L, 333333L, 999999L};
         short[] arr7 = {-3, 0, 3};
+        short[] arr7_custom = {-3, 0, 3};
+        short[] arr7_faulty = {-3, 0, 3};
         BigInteger num = BigInteger.valueOf(3);
         BigInteger den = BigInteger.valueOf(5);
 
         DafnyVMC.Random r = new DafnyVMC.Random();
-        Uniform.Interface.Trait t = new CustomUniformSample();
-        Uniform.Interface.Trait t_faulty = new CustomUniformSampleFaulty();
+        CustomFisherYates r_custom = new CustomFisherYates();
+        CustomFisherYatesFaulty r_faulty = new CustomFisherYatesFaulty();
 
         System.out.println("Example of Uniform sampling");
         System.out.println(r.UniformSample(BigInteger.valueOf(4)));
@@ -43,60 +51,84 @@ public class BuildTest {
         System.out.println(Arrays.toString(arr1));
 
         System.out.println("Example of custom Fisher-Yates: BigInteger");
-        r.Shuffle(arr1, t);
-        System.out.println(Arrays.toString(arr1));
+        r_custom.Shuffle(arr1_custom);
+        System.out.println(Arrays.toString(arr1_custom));
 
         System.out.println("Example of faulty custom Fisher-Yates: BigInteger");
-        r.Shuffle(arr1b, t_faulty);
-        System.out.println(Arrays.toString(arr1b));
+        r_faulty.Shuffle(arr1_faulty);
+        System.out.println(Arrays.toString(arr1_faulty));
  
         System.out.println("Example of Fisher-Yates: int");
         r.Shuffle(arr2);
         System.out.println(Arrays.toString(arr2));
 
         System.out.println("Example of custom Fisher-Yates: int");
-        r.Shuffle(arr2, t);
-        System.out.println(Arrays.toString(arr2));
+        r_custom.Shuffle(arr2_custom);
+        System.out.println(Arrays.toString(arr2_custom));
+
+        System.out.println("Example of faulty custom Fisher-Yates: int");
+        r_faulty.Shuffle(arr2_faulty);
+        System.out.println(Arrays.toString(arr2_faulty));
 
         System.out.println("Example of Fisher-Yates: String");
         r.Shuffle(arr3);
         System.out.println(Arrays.toString(arr3));
 
         System.out.println("Example of custom Fisher-Yates: String");
-        r.Shuffle(arr3, t);
-        System.out.println(Arrays.toString(arr3));
+        r_custom.Shuffle(arr3_custom);
+        System.out.println(Arrays.toString(arr3_custom));
+
+        System.out.println("Example of faulty custom Fisher-Yates: String");
+        r_faulty.Shuffle(arr3_faulty);
+        System.out.println(Arrays.toString(arr3_faulty));
 
         System.out.println("Example of Fisher-Yates: char");
         r.Shuffle(arr4);
         System.out.println(Arrays.toString(arr4));
 
         System.out.println("Example of custom Fisher-Yates: char");
-        r.Shuffle(arr4, t);
-        System.out.println(Arrays.toString(arr4));
+        r_custom.Shuffle(arr4_custom);
+        System.out.println(Arrays.toString(arr4_custom));
+
+        System.out.println("Example of faulty custom Fisher-Yates: char");
+        r_faulty.Shuffle(arr4_faulty);
+        System.out.println(Arrays.toString(arr4_faulty));
 
         System.out.println("Example of Fisher-Yates: boolean");
         r.Shuffle(arr5);
         System.out.println(Arrays.toString(arr5));
 
         System.out.println("Example of custom Fisher-Yates: boolean");
-        r.Shuffle(arr5, t);
-        System.out.println(Arrays.toString(arr5));
+        r_custom.Shuffle(arr5_custom);
+        System.out.println(Arrays.toString(arr5_custom));
+
+        System.out.println("Example of faulty custom Fisher-Yates: boolean");
+        r_faulty.Shuffle(arr5_faulty);
+        System.out.println(Arrays.toString(arr5_faulty));
 
         System.out.println("Example of Fisher-Yates: long");
         r.Shuffle(arr6);
         System.out.println(Arrays.toString(arr6));
 
         System.out.println("Example of custom Fisher-Yates: long");
-        r.Shuffle(arr6, t);
-        System.out.println(Arrays.toString(arr6));
+        r_custom.Shuffle(arr6_custom);
+        System.out.println(Arrays.toString(arr6_custom));
+
+        System.out.println("Example of faulty custom Fisher-Yates: long");
+        r_faulty.Shuffle(arr6_faulty);
+        System.out.println(Arrays.toString(arr6_faulty));
 
         System.out.println("Example of Fisher-Yates: short");
         r.Shuffle(arr7);
         System.out.println(Arrays.toString(arr7));
 
         System.out.println("Example of custom Fisher-Yates: short");
-        r.Shuffle(arr7, t);
-        System.out.println(Arrays.toString(arr7));
+        r_custom.Shuffle(arr7_custom);
+        System.out.println(Arrays.toString(arr7_custom));
+
+        System.out.println("Example of faulty custom Fisher-Yates: short");
+        r_faulty.Shuffle(arr7_faulty);
+        System.out.println(Arrays.toString(arr7_faulty));
     }
 }
 
