docs/java/CustomFisherYates.java
@@ -3,6 +3,7 @@ import Uniform.Interface.Trait;
 import java.math.BigInteger;
 import java.security.SecureRandom;
 import java.util.Random;
+import dafny.TypeDescriptor;
 
 class CustomUniformSampleMinus implements Uniform.Interface.TraitMinus {
   static ThreadLocal<SecureRandom> rng;
@@ -40,8 +41,49 @@ class CustomUniformSampleMinus implements Uniform.Interface.TraitMinus {
   }
 }
 
-public class CustomUniformSample extends CustomUniformSampleMinus implements Uniform.Interface.Trait {
+class CustomUniform extends CustomUniformSampleMinus implements Uniform.Interface.Trait {
   public java.math.BigInteger UniformIntervalSample(java.math.BigInteger a, java.math.BigInteger b) {
     return Uniform.Interface._Companion_Trait.UniformIntervalSample(this, a, b);
+  }
+}
+
+
+class CustomFisherYatesMinus extends CustomUniform implements FisherYates.Implementation.Trait {
+  public <__T> void Shuffle(dafny.TypeDescriptor<__T> _td___T, java.lang.Object a) {
+    FisherYates.Implementation._Companion_Trait.Shuffle(_td___T, this, a);
+  }
+
+  public <__T> void Swap(dafny.TypeDescriptor<__T> _td___T, java.lang.Object a, java.math.BigInteger i, java.math.BigInteger j) {
+    FisherYates.Implementation._Companion_Trait.Swap(_td___T, this, a, i, j);
+  }
+}
+
+public class CustomFisherYates extends CustomFisherYatesMinus {
+  public void Shuffle(BigInteger[] arr) {
+    this.Shuffle(TypeDescriptor.BIG_INTEGER, arr);
+  }
+
+  public void Shuffle(int[] arr) {
+    this.Shuffle(TypeDescriptor.INT, arr);
+  }
+
+  public void Shuffle(String[] arr) {
+    this.Shuffle(TypeDescriptor.CHAR_ARRAY, arr);
+  }
+
+  public void Shuffle(char[] arr) {
+    this.Shuffle(TypeDescriptor.CHAR, arr);
+  }
+
+  public void Shuffle(boolean[] arr) {
+    this.Shuffle(TypeDescriptor.BOOLEAN, arr);
+  }
+
+  public void Shuffle(long[] arr) {
+    this.Shuffle(TypeDescriptor.LONG, arr);
+  }
+
+  public void Shuffle(short[] arr) {
+    this.Shuffle(TypeDescriptor.SHORT, arr);
   }
 }
