build/java/run.sh
@@ -1,3 +1,3 @@
 #1/bin/bash
-javac -classpath "build/java/DafnyVMC.jar:docs/java/" docs/java/CustomUniformSample.java docs/java/CustomUniformSampleFaulty.java
+javac -classpath "build/java/DafnyVMC.jar:docs/java/" docs/java/CustomFisherYates.java docs/java/CustomFisherYatesFaulty.java
 java -classpath "build/java/DafnyVMC.jar:docs/java/" docs/java/BuildTest.java 
